symbolic/backward.v
@@ -218,8 +218,7 @@ Proof.
 Qed.
 
 Lemma initial_handler_state cst kst cmvec cmem' :
-  forall (ISUSER : in_user cst)
-         (CMVEC : build_cmvec _ cst = Some cmvec)
+  forall (CMVEC : build_cmvec cst = Some cmvec)
          (MEM : Concrete.store_mvec (Concrete.mem cst) cmvec = Some cmem')
          (MISS : Concrete.cache_lookup (Concrete.cache cst) masks cmvec = None)
          (STEP : Concrete.step _ masks cst kst),
@@ -229,26 +228,10 @@ Lemma initial_handler_state cst kst cmvec cmem' :
                              (Concrete.fault_handler_start mt)@Concrete.TKernel
                              (Concrete.pc cst).
 Proof.
-  intros.
-  rewrite (lock build_cmvec) in CMVEC.
-  inv STEP; try subst mvec;
-  unfold Concrete.next_state_reg, Concrete.next_state_reg_and_pc,
-         Concrete.next_state_pc, Concrete.next_state,
-         Concrete.miss_state in *;
-  match_inv; simpl in *.
-
-  analyze_cache.
-  try analyze_cache; simpl in *.
-
-  solve [
-    repeat simpl_word_lift; simpl in *; discriminate |
-    move: CMVEC;
-    rewrite -(lock build_cmvec) /=;
-    repeat match goal with
-           | E : ?X = _ |- context [?X] => rewrite E; simpl
-           end;
-    congruence
-  ].
+  move=> BUILD MVEC LOOKUP /step_lookup_success_or_fault.
+  rewrite BUILD.
+  case=> [cmvec' [[<-]]] {cmvec'}.
+  by rewrite LOOKUP MVEC.
 Qed.
 
 Lemma kernel_user_exec_determ k s1 s2 :
@@ -260,8 +243,8 @@ Proof.
   eapply exec_until_determ; eauto.
   - clear. intros s s1 s2.
     do 2 rewrite <- stepP in *. congruence.
-  - clear. intros s H1 H2. simpl in *. congruence.
-  - clear. intros s H1 H2. simpl in *. congruence.
+  - clear. by move=> s /= ->.
+  - clear. by move=> s /= ->.
 Qed.
 
 Lemma user_kernel_user_step_determ s s1 s2 :
@@ -278,30 +261,15 @@ Import Vector.VectorNotations.
 
 Lemma build_cmvec_cache_lookup_pc cst cst' cmvec crvec :
   Concrete.step _ masks cst cst' ->
-  build_cmvec _ cst = Some cmvec ->
+  build_cmvec cst = Some cmvec ->
   Concrete.cache_lookup (Concrete.cache cst) masks cmvec = Some crvec ->
   common.tag (Concrete.pc cst') = Concrete.ctrpc crvec.
 Proof.
-  move/stepP.
-  case: cst => mem regs cache [pc tpc] epc /= STEP BUILD LOOKUP.
-  move: BUILD STEP.
-  case: (PartMaps.get mem pc) => [[w ti]|] //=.
-  case: (decode_instr w) => [i|] //=.
-  destruct i => BUILD STEP; repeat match_inv;
-  unfold Concrete.next_state_pc, Concrete.next_state_reg,
-         Concrete.next_state_reg_and_pc, Concrete.next_state in *;
-  simpl in *;
-  repeat match goal with
-  | E1 : ?x = ?y1, E2 : ?x = ?y2 |- _ =>
-   rewrite E1 in E2; inv E2
-  end;
-  try match goal with
-  | LOOKUP : Concrete.cache_lookup _ _ _ = Some _,
-    STEP : context[Concrete.cache_lookup _ _ _] |- _ =>
-    rewrite LOOKUP in STEP
-  end;
-  match_inv; simpl; trivial.
-  discriminate.
+  move=> STEP BUILD LOOKUP.
+  move/step_lookup_success_or_fault: STEP.
+  rewrite BUILD.
+  case=> cmvec' [[<-]] {cmvec'}.
+  by rewrite LOOKUP.
 Qed.
 
 Lemma kernel_cache_lookup_fail (cst cst' : Concrete.state mt) cmvec :
@@ -310,52 +278,29 @@ Lemma kernel_cache_lookup_fail (cst cst' : Concrete.state mt) cmvec :
   Concrete.step _ masks cst cst' ->
   ~~ cache_allows_syscall table cst ->
   wf_entry_points table (Concrete.mem cst) ->
-  cache_correct (Concrete.cache cst) ->
-  build_cmvec _ cst = Some cmvec ->
+  cache_correct (Concrete.cache cst) (Concrete.mem cst) ->
+  build_cmvec cst = Some cmvec ->
   Concrete.cache_lookup (Concrete.cache cst) masks cmvec = None.
 Proof.
-  case: cst => mem regs cache [pc tpc] epc.
   move=> INUSER INKERNEL STEP NOTALLOWED WFENTRYPOINTS CACHECORRECT BUILD.
-  move: NOTALLOWED.
-  rewrite /cache_allows_syscall /=.
-  case GETSC: (Symbolic.get_syscall table pc) => [sc|] //=.
-    case LOOKUP: (Concrete.cache_lookup cache masks _) => [res|] //= _.
-    rewrite <- LOOKUP. apply f_equal.
-    move: BUILD.
-    rewrite /build_cmvec.
-    have [i [-> /is_nopP -> //=]] := wf_entry_points_if _ WFENTRYPOINTS GETSC.
-    congruence.
-  case LOOKUP: (Concrete.cache_lookup cache masks _) => [crvec|] //= _.
-  have E: Concrete.ctrpc crvec = Concrete.TKernel.
-    move: INKERNEL.
-    rewrite -(build_cmvec_cache_lookup_pc STEP BUILD LOOKUP)
-             /in_kernel /Concrete.is_kernel_tag.
-    by move/eqP.
-  move/(_ cmvec crvec): CACHECORRECT. move: INUSER.
-  rewrite (build_cmvec_ctpc _ _ _ BUILD) /= /in_user /=
-          => INUSER /(_ INUSER LOOKUP) {INUSER} [ivec [ovec [? [? _]]]].
-  subst cmvec crvec.
-  suff: false by done.
-  move: E.
-  rewrite /encode_ovec /ovec_of_uovec /=.
-  have [E _|NE /=] := Symbolic.op ivec =P SERVICE; last first.
-    rewrite (@encode_kernel_tag _ (Symbolic.ttypes Symbolic.P) _).
-    by move=> /encode_inj.
-  move=> {LOOKUP}.
-  have [//= i [instr [Hi Hinstr /op_to_word_inj Hinstr']]] := build_cmvec_cop_cti _ _ _ BUILD.
-  have [ISNOP [t Ht]] : opcode_of instr = NOP /\ exists t, Symbolic.ti (ivec_of_uivec ivec) = ENTRY t.
-    rewrite {}Hinstr'.
-    move: E {BUILD Hi ovec}.
-    case: ivec => op tpc' ti ts /= H.
-    move: ts.
-    by rewrite {}H=> _ /=; eauto.
-  rewrite {}Ht in Hi.
-  move: ISNOP {Hinstr'} Hinstr.
-  case: instr => //= _ Hinstr.
-  move: (WFENTRYPOINTS pc t) => /=.
-  rewrite Hi eqxx /is_nop Hinstr /= => {E} E.
-  move/E: (erefl true) => [? [? ?]].
-  congruence.
+  move/step_lookup_success_or_fault: STEP NOTALLOWED.
+  rewrite /cache_allows_syscall BUILD.
+  case=> cmvec' [[<-]] {cmvec'}.
+  case LOOKUP: (Concrete.cache_lookup _ _ _) => [[ctrpc ctr]|] //= E. subst ctrpc.
+  case GETSC: (Symbolic.get_syscall _ _) => [sc|] //=.
+  move: INKERNEL LOOKUP.
+  rewrite /in_kernel /Concrete.is_kernel_tag => /eqP -> LOOKUP _.
+  rewrite /in_user -(build_cmvec_ctpc BUILD) in INUSER.
+  case/(_ cmvec _ LOOKUP INUSER): CACHECORRECT => ivec [ovec [/decode_ivec_inv DECi DECo _ _]].
+  case: DECi ovec DECo => [[op [E DEC _ _ _]]|[DECop E _ DECti]].
+    by rewrite {}E {ivec} /decode_ovec /= decode_kernel_tag /= => ovec.
+  suff : false by done.
+  move: {ivec E} (Symbolic.ti ivec) DECti => ti DECti.
+  move: (build_cmvec_cop_cti BUILD) DECop => [i [instr [GETPC DECi <-]]].
+  rewrite op_to_wordK => [[Hinstr]].
+  have {DECi Hinstr} ISNOP : is_nop i by rewrite /is_nop {}DECi; case: instr Hinstr.
+  move: (wf_entry_points_only_if WFENTRYPOINTS GETPC DECti ISNOP).
+  rewrite GETSC. by case=> ? [? ?].
 Qed.
 
 Lemma cache_miss_simulation sst cst cst' :
@@ -367,43 +312,48 @@ Proof.
   move => REF NOTALLOWED [kst ISUSER STEP KEXEC].
   have KER : in_kernel kst = true.
   { destruct KEXEC as [? EXEC]. exact (restricted_exec_fst EXEC). }
-  destruct REF as [smem sregs int cmem cregs cache epc pc tpc
-                   ? ? REFM REFR CACHECORRECT  MVEC WFENTRYPOINTS KINV].
+  destruct REF as [smem sregs int cmem cregs cache epc pc ctpc tpc
+                   ? ? DEC REFM REFR CACHECORRECT MVEC WFENTRYPOINTS KINV].
   subst sst cst.
-  assert (NUSER : @word_lift _ _ (e Symbolic.P) (fun t => is_user t) (common.tag (Concrete.pc kst)) = false).
-  { destruct (@word_lift _ _ (e Symbolic.P) (fun t => is_user t) (common.tag (Concrete.pc kst))) eqn:EQ; trivial.
-    rewrite /in_kernel in KER.
-    apply is_user_pc_tag_is_kernel_tag in EQ; auto. congruence. }
-  have [cmvec Hcmvec] := step_build_cmvec _ _ _ _ STEP.
+  have ISUSER' : ~~ in_kernel cst' by case: KEXEC.
+  have [cmvec Hcmvec] := step_build_cmvec STEP.
   have [cmem' Hcmem'] := mvec_in_kernel_store_mvec cmvec MVEC.
   have LOOKUP := kernel_cache_lookup_fail ISUSER KER STEP NOTALLOWED WFENTRYPOINTS CACHECORRECT Hcmvec.
-  have H := initial_handler_state ISUSER Hcmvec Hcmem' LOOKUP STEP.
-  subst. simpl in *.
-  case HANDLER: (handler _ (fun m => Symbolic.transfer m) cmvec) => [rvec|].
-  - destruct (handler_correct_allowed_case cmem cmvec cregs pc@(encode (USER tpc)) int
-                                           KINV HANDLER Hcmem' CACHECORRECT)
-      as (cst'' & KEXEC' & CACHE' & LOOKUP' & MVEC' &
+  have H := initial_handler_state Hcmvec Hcmem' LOOKUP STEP.
+  have EXEC : exec (Concrete.step _ masks) kst cst'.
+    case: KEXEC => kst' EXEC _ STEP'.
+    apply restricted_exec_weaken in EXEC.
+    by apply restricted_exec_trans with kst'; eauto.
+  subst kst. rewrite /= in STEP KEXEC EXEC KER LOOKUP.
+  case DECivec: (decode_ivec _ cmem cmvec) => [ivec|]; last first.
+    have := (handler_correct_disallowed_case KINV _ Hcmem' ISUSER' EXEC).
+    move=> /(_ _ kcc). by rewrite DECivec => /(_ erefl).
+  case TRANS: (Symbolic.transfer ivec) => [ovec|]; last first.
+    have := (handler_correct_disallowed_case KINV _ Hcmem' ISUSER' EXEC).
+    move=> /(_ _ kcc). by rewrite DECivec TRANS => /(_ erefl).
+  destruct (handler_correct_allowed_case pc@ctpc KINV DECivec TRANS Hcmem' CACHECORRECT)
+      as (cst'' & rvec & KEXEC' & CACHE' & LOOKUP' & DECovec & MVEC' &
           HMEM & HREGS & HPC & WFENTRYPOINTS' & KINV').
-    assert (EQ := kernel_user_exec_determ KEXEC' KEXEC). subst cst''.
-    destruct cst' as [cmem'' cregs'' cache' ? ?]. simpl in *. subst.
-    econstructor; eauto.
-    + clear - ISUSER MVEC Hcmem' REFM HMEM.
-      intros addr w t. unfold user_mem_unchanged in *.
-      rewrite <- HMEM. apply REFM.
-    + clear - REFR HREGS.
-      intros r w t. unfold user_regs_unchanged in *.
-      rewrite <- HREGS.
-      apply REFR.
-  - assert (EXEC : forall st st',
-                     kernel_user_exec st st' ->
-                     exec (Concrete.step _ masks) st st').
-    { clear. intros st st' EXEC. destruct EXEC as [kst' EXEC].
-      apply restricted_exec_weaken in EXEC.
-      apply restricted_exec_trans with kst'; eauto. }
-    assert (ISUSER' : in_kernel cst' = false).
-    { destruct KEXEC. eauto. }
-    apply EXEC in KEXEC.
-    destruct (handler_correct_disallowed_case cmem cmvec int KINV HANDLER Hcmem' ISUSER' KEXEC).
+  have EQ := kernel_user_exec_determ KEXEC' KEXEC. subst cst''.
+  case: cst' {KEXEC KEXEC' EXEC LOOKUP' DECovec} HPC CACHE'
+             ISUSER' MVEC' HMEM HREGS WFENTRYPOINTS' KINV' =>
+        cmem'' cregs'' cache' pc' ? /= -> {pc'} CACHE' ISUSER' MVEC' HMEM HREGS WFENTRYPOINTS' KINV'.
+  econstructor; eauto.
+  - admit.
+  - split.
+    + move=> w x ctg atg {DECivec DEC} DEC GET.
+      move: (HMEM w x ctg atg) => [_ /(_ (conj GET DEC)) {GET DEC} [GET DEC]].
+      by eapply (proj1 REFM); eauto.
+    + move=> w x atg /(proj2 REFM) {DEC} [ctg DEC GET].
+      move: (HMEM w x ctg atg) => [/(_ (conj GET DEC)) {GET DEC} [GET DEC] _].
+      by eauto.
+  - split.
+    + move=> r x ctg atg {DECivec DEC} DEC GET.
+      move: (HREGS r x ctg atg) => [_ /(_ (conj GET DEC)) {GET DEC} [GET DEC]].
+      by eapply (proj1 REFR); eauto.
+    + move=> r x atg /(proj2 REFR) {DEC} [ctg DEC GET].
+      move: (HREGS r x ctg atg) => [/(_ (conj GET DEC)) {GET DEC} [GET DEC] _].
+      by eauto.
 Qed.
 
 Lemma syscall_simulation sst cst cst' :
@@ -414,8 +364,8 @@ Lemma syscall_simulation sst cst cst' :
                refine_state ki table sst' cst'.
 Proof.
   intros REF ALLOWED STEP.
-  destruct REF as [smem sregs int cmem cregs cache epc pc tpc
-                   ? ? REFM REFR CACHE MVEC WFENTRYPOINTS KINV].
+  destruct REF as [smem sregs int cmem cregs cache epc pc ctpc tpc
+                   ? ? DEC REFM REFR CACHE MVEC WFENTRYPOINTS KINV].
   subst sst cst.
   have [sc GETCALL]: (exists sc, Symbolic.get_syscall table pc = Some sc).
   { rewrite /cache_allows_syscall in ALLOWED.
@@ -424,44 +374,36 @@ Proof.
   case SCEXEC: (Symbolic.run_syscall sc (Symbolic.State smem sregs pc@tpc int))
     => [[smem' sregs' [pc' tpc'] int']|].
   - exploit syscalls_correct_allowed_case; eauto.
-    intros (cmem' & creg' & cache' & pct' & EXEC' &
+    intros (cmem' & creg' & cache' & ctpc' & epc' & EXEC' &
             REFM' & REFR' & CACHE' & MVEC' & WFENTRYPOINTS' & KINV').
     generalize (user_kernel_user_step_determ STEP EXEC'). intros ?. subst.
     { exists (Symbolic.State smem' sregs' pc'@tpc' int'). split.
       - eapply Symbolic.step_syscall; eauto.
         eapply wf_entry_points_if in GETCALL; last by exact WFENTRYPOINTS.
-        move: GETCALL => [i [GETPC ISNOP]].
+        move: GETCALL => [i [ti [GETPC DECti ISNOP]]].
         case GET': (PartMaps.get smem pc) => [[? ?]|] //.
-        move/REFM: GET' => GET'.
+        move: (proj2 REFM _ _ _ GET') => {GET' DEC} [ctg' DEC GET'].
         rewrite GETPC in GET'.
-        move: GET' => [? H].
-        by apply encode_inj in H.
-      - econstructor; eauto. }
-  - destruct (syscalls_correct_disallowed_case _ _ KINV REFM REFR CACHE MVEC
-                                               WFENTRYPOINTS GETCALL SCEXEC ALLOWED STEP).
+        move: GET' => [? H]. subst i ti.
+        by rewrite DEC in DECti.
+      - econstructor; eauto.
+        admit. }
+  - destruct (syscalls_correct_disallowed_case KINV REFM REFR CACHE MVEC
+                                               WFENTRYPOINTS GETCALL SCEXEC DEC ALLOWED STEP).
 Qed.
 
 Lemma user_into_kernel sst cst cst' :
   refine_state ki table sst cst ->
   Concrete.step _ masks cst cst' ->
-  in_user cst' = false ->
-  in_kernel cst' = true.
+  ~~ in_user cst'->
+  in_kernel cst'.
 Proof.
-  intros REF STEP NUSER.
+  move=> REF STEP NUSER.
   move: (refine_state_in_user REF) => INUSER.
-  destruct (in_kernel cst') eqn:NKERNEL; trivial.
-  unfold in_user in NUSER.
-  unfold in_kernel, Concrete.is_kernel_tag in NKERNEL.
-  rewrite (@encode_kernel_tag _ _ (e Symbolic.P)) in NKERNEL.
-  destruct REF as [? ? ? ? ? ? ? ? ? ? ? ? ? CACHE ? ? ?].
-  subst sst cst.
-  assert (PCS := valid_pcs STEP CACHE INUSER).
-  rewrite /word_lift in NUSER.
-  destruct (decode (common.tag (Concrete.pc cst'))) as [[t| |]|] eqn:DEC;
-  try discriminate; simpl in *;
-  apply encodeK in DEC.
-  rewrite <- DEC in NKERNEL.
-  rewrite eq_tag_eq_word // in NKERNEL.
+  case: REF => [? ? ? ? ? ? ? ? ? ? ? ? ? ? ? CACHE ? ? ?]. subst.
+  move : (valid_pcs STEP CACHE INUSER) NUSER.
+  rewrite /in_kernel /Concrete.is_kernel_tag /in_user.
+  move => [[t ->]|->] //=.
 Qed.
 
 Definition refine_state_weak sst cst :=
@@ -480,20 +422,20 @@ Lemma backwards_simulation sst cst cst' :
     refine_state ki table sst' cst'.
 Proof.
   intros [REF | (cst0 & kst & REF & KSTEP & EXEC)] STEP.
-  - assert (USER : in_user cst = true) by (eapply refine_state_in_user; eauto).
-    destruct (in_user cst') eqn:USER'.
+  - have USER : in_user cst by eapply refine_state_in_user; eauto.
+    have [USER'|USER'] := boolP (in_user cst').
     + right.
       eapply cache_hit_simulation; eauto.
       by constructor; auto.
     + left. right. do 2 eexists. do 2 (split; eauto).
       constructor.
       by eapply user_into_kernel; eauto.
-  - assert (USER : in_user cst0 = true) by (eapply refine_state_in_user; eauto).
-    destruct (in_kernel cst') eqn:KER'.
+  - have USER : in_user cst0 by eapply refine_state_in_user; eauto.
+    have [KER'|KER'] := boolP (in_kernel cst').
     + left. right.
       do 2 eexists. do 2 (split; eauto).
       eapply restricted_exec_trans; eauto.
-      have KER : in_kernel cst = true by eapply restricted_exec_snd in EXEC.
+      have KER : in_kernel cst by eapply restricted_exec_snd in EXEC.
       eapply re_step; by eauto using user_into_kernel.
     + assert (EXEC' : user_kernel_user_step cst0 cst').
       { econstructor; eauto.
@@ -506,7 +448,7 @@ Qed.
 Theorem backwards_refinement sst cst cst' :
   refine_state ki table sst cst ->
   exec (Concrete.step _ masks) cst cst' ->
-  in_user cst' = true ->
+  in_user cst' ->
   exists sst',
     exec (Symbolic.step table) sst sst' /\
     refine_state ki table sst' cst'.
@@ -518,7 +460,8 @@ Proof.
   - move => sst [? | REF]; first by eauto.
     destruct REF as (? & ? & ? & ? & EXEC).
     apply restricted_exec_snd in EXEC.
-    apply in_user_in_kernel in USER'. congruence.
+    apply in_user_in_kernel in USER'.
+    by rewrite EXEC in USER'.
   - move => sst REF.
     exploit backwards_simulation; eauto.
     intros [REF' | (sst' & SSTEP & REF')]; first by auto.
